lean4/ProofChecker/ProofChecker/PropTerm.lean
@@ -1,0 +1,173 @@
+/-
+Copyright (c) 2023 Wojciech Nawrocki. All rights reserved.
+Released under Apache 2.0 license as described in the file LICENSE.
+Authors: Wojciech Nawrocki
+-/
+
+import ProofChecker.PropForm
+
+/-! The term model of propositional formulas. We show that it is a Heyting algebra. -/
+
+open PropForm in
+instance PropTerm.setoid (ν : Type) : Setoid (PropForm ν) where
+  r := equivalent
+  iseqv := {
+    refl  := equivalent_refl
+    symm  := equivalent.symm
+    trans := equivalent.trans
+  }
+
+/-- A propositional term is a propositional formula up to semantic equivalence. -/
+def PropTerm ν := Quotient (PropTerm.setoid ν)
+
+namespace PropTerm
+
+def var (x : ν) : PropTerm ν := ⟦.var x⟧
+
+def tr : PropTerm ν := ⟦.tr⟧
+
+def fls : PropTerm ν := ⟦.fls⟧
+
+def neg : PropTerm ν → PropTerm ν :=
+  Quotient.map (.neg ·) (by
+    intro _ _ h _ _ τ
+    simp [h τ])
+
+def conj : PropTerm ν → PropTerm ν → PropTerm ν := 
+  Quotient.map₂ (.conj · ·) (by
+    intro _ _ h₁ _ _ h₂ _ _ τ
+    simp [h₁ τ, h₂ τ])
+
+def disj : PropTerm ν → PropTerm ν → PropTerm ν :=
+  Quotient.map₂ (.disj · ·) (by
+    intro _ _ h₁ _ _ h₂ _ _ τ
+    simp [h₁ τ, h₂ τ])
+
+def impl : PropTerm ν → PropTerm ν → PropTerm ν :=
+  Quotient.map₂ (.impl · ·) (by
+    intro _ _ h₁ _ _ h₂ _ _ τ
+    simp [h₁ τ, h₂ τ])
+
+def biImpl : PropTerm ν → PropTerm ν → PropTerm ν :=
+  Quotient.map₂ (.biImpl · ·) (by
+    intro _ _ h₁ _ _ h₂ _ _ τ
+    simp [h₁ τ, h₂ τ])
+
+def entails : PropTerm ν → PropTerm ν → Prop :=
+  Quotient.lift₂ (PropForm.entails · ·) (by
+    intro _ _ _ _ h₁ h₂
+    dsimp [HasEquiv.Equiv, Setoid.r, PropForm.equivalent] at h₁ h₂
+    simp [PropForm.entails, h₁, h₂])
+
+-- TODO: All of these just lift the corresponding lemmas from PropFrom, is there a quicker way?
+
+theorem entails_refl (φ : PropTerm ν) : entails φ φ := by
+  have ⟨φ, h⟩ := Quotient.exists_rep φ
+  simp [← h, entails, PropForm.entails]
+
+theorem entails.trans : entails φ ψ → entails ψ θ → entails φ θ := by
+  have ⟨φ, h₁⟩ := Quotient.exists_rep φ
+  have ⟨ψ, h₂⟩ := Quotient.exists_rep ψ
+  have ⟨θ, h₃⟩ := Quotient.exists_rep θ
+  simp only [← h₁, ← h₂, ← h₃]
+  exact PropForm.entails.trans
+
+theorem entails.antisymm : entails φ ψ → entails ψ φ → φ = ψ := by
+  have ⟨φ, h₁⟩ := Quotient.exists_rep φ
+  have ⟨ψ, h₂⟩ := Quotient.exists_rep ψ
+  simp only [← h₁, ← h₂, entails, Quotient.lift₂_mk]
+  rw [Quotient.eq]
+  exact PropForm.entails.antisymm
+
+theorem entails_tr (φ : PropTerm ν) : entails φ tr := by
+  have ⟨φ, h⟩ := Quotient.exists_rep φ
+  simp [← h, entails, tr, PropForm.entails_tr]
+
+theorem fls_entails (φ : PropTerm ν) : entails fls φ := by
+  have ⟨φ, h⟩ := Quotient.exists_rep φ
+  simp [← h, entails, fls, PropForm.fls_entails]
+
+theorem entails_disj_left (φ ψ : PropTerm ν) : entails φ (disj φ ψ) := by
+  have ⟨φ, h₁⟩ := Quotient.exists_rep φ
+  have ⟨ψ, h₂⟩ := Quotient.exists_rep ψ
+  simp [← h₁, ← h₂, entails, disj, PropForm.entails_disj_left]
+
+theorem entails_disj_right (φ ψ : PropTerm ν) : entails ψ (disj φ ψ) := by
+  have ⟨φ, h₁⟩ := Quotient.exists_rep φ
+  have ⟨ψ, h₂⟩ := Quotient.exists_rep ψ
+  simp [← h₁, ← h₂, entails, disj, PropForm.entails_disj_right]
+
+theorem disj_entails : entails φ θ → entails ψ θ → entails (disj φ ψ) θ := by
+  have ⟨φ, h₁⟩ := Quotient.exists_rep φ
+  have ⟨ψ, h₂⟩ := Quotient.exists_rep ψ
+  have ⟨θ, h₃⟩ := Quotient.exists_rep θ
+  simp only [← h₁, ← h₂, ← h₃, entails, disj, Quotient.lift₂_mk, Quotient.map₂_mk]
+  exact PropForm.disj_entails
+
+theorem conj_entails_left (φ ψ : PropTerm ν) : entails (conj φ ψ) φ := by
+  have ⟨φ, h₁⟩ := Quotient.exists_rep φ
+  have ⟨ψ, h₂⟩ := Quotient.exists_rep ψ
+  simp [← h₁, ← h₂, entails, conj, PropForm.conj_entails_left]
+
+theorem conj_entails_right (φ ψ : PropTerm ν) : entails (conj φ ψ) ψ := by
+  have ⟨φ, h₁⟩ := Quotient.exists_rep φ
+  have ⟨ψ, h₂⟩ := Quotient.exists_rep ψ
+  simp [← h₁, ← h₂, entails, conj, PropForm.conj_entails_right]
+
+theorem entails_conj : entails φ ψ → entails φ θ → entails φ (conj ψ θ) := by
+  have ⟨φ, h₁⟩ := Quotient.exists_rep φ
+  have ⟨ψ, h₂⟩ := Quotient.exists_rep ψ
+  have ⟨θ, h₃⟩ := Quotient.exists_rep θ
+  simp only [← h₁, ← h₂, ← h₃, entails, conj, Quotient.lift₂_mk, Quotient.map₂_mk]
+  exact PropForm.entails_conj
+
+theorem entails_impl_iff (φ ψ θ : PropTerm ν) : entails φ (impl ψ θ) ↔ entails (conj φ ψ) θ := by
+  have ⟨φ, h₁⟩ := Quotient.exists_rep φ
+  have ⟨ψ, h₂⟩ := Quotient.exists_rep ψ
+  have ⟨θ, h₃⟩ := Quotient.exists_rep θ
+  simp [← h₁, ← h₂, ← h₃, entails, impl, conj, PropForm.entails_impl_iff]
+
+theorem impl_fls (φ : PropTerm ν) : impl φ fls = neg φ := by
+  have ⟨φ, h₁⟩ := Quotient.exists_rep φ
+  simp only [← h₁, impl, fls, neg, Quotient.map_mk, Quotient.map₂_mk]
+  rw [Quotient.eq]
+  exact PropForm.impl_fls φ
+
+theorem conj_neg_entails_fls (φ : PropTerm ν) : entails (conj φ (neg φ)) fls := by
+  have ⟨φ, h₁⟩ := Quotient.exists_rep φ
+  simp [← h₁, entails, conj, neg, fls, PropForm.conj_neg_entails_fls]
+
+theorem tr_entails_disj_neg (φ : PropTerm ν) : entails tr (disj φ (neg φ)) := by
+  have ⟨φ, h₁⟩ := Quotient.exists_rep φ
+  simp [← h₁, entails, tr, disj, neg, PropForm.tr_entails_disj_neg]
+
+theorem entails_disj_conj (φ ψ θ : PropTerm ν) :
+    entails (conj (disj φ ψ) (disj φ θ)) (disj φ (conj ψ θ)) := by
+  have ⟨φ, h₁⟩ := Quotient.exists_rep φ
+  have ⟨ψ, h₂⟩ := Quotient.exists_rep ψ
+  have ⟨θ, h₃⟩ := Quotient.exists_rep θ
+  simp [← h₁, ← h₂, ← h₃, entails, conj, disj, PropForm.entails_disj_conj]
+
+instance : BooleanAlgebra (PropTerm ν) where
+  le := entails
+  top := tr
+  bot := fls
+  compl := neg
+  sup := disj
+  inf := conj
+  le_refl := entails_refl
+  le_trans := @entails.trans _
+  le_antisymm := @entails.antisymm _
+  le_top := entails_tr
+  bot_le := fls_entails
+  le_sup_left := entails_disj_left
+  le_sup_right := entails_disj_right
+  sup_le _ _ _ := disj_entails
+  inf_le_left := conj_entails_left
+  inf_le_right := conj_entails_right
+  le_inf _ _ _ := entails_conj
+  le_sup_inf := entails_disj_conj
+  inf_compl_le_bot := conj_neg_entails_fls
+  top_le_sup_compl := tr_entails_disj_neg
+
+end PropTerm
